Dex001/README.md
@@ -1,2 +1,5 @@
 
-To verify, run `zebra  --z3rlimit 8000000 -v Dex001.fst`.  
+To verify/record hints, run `zebra  --z3rlimit 4500000 -v Dex001.fst`.  
+This command may take a long time to run the first time.
+Subsequent runs will be significantly faster.
+With an AMD Threadripper 1950x @4.0GHz, recording hints takes ~67s. Subsequent runs take ~11s.
